Updates

generic/Zeta.Generic.Global.fsti
@@ -4,6 +4,7 @@ open FStar.Seq
 open Zeta.SeqAux
 open Zeta.Interleave
 open Zeta.Time
+open Zeta.InterleaveMultiSet
 open Zeta.MultiSetHashDomain
 open Zeta.GenericVerifier
 open Zeta.Generic.Thread
@@ -12,6 +13,7 @@ module S = FStar.Seq
 module SA = Zeta.SeqAux
 module T = Zeta.Generic.Thread
 module I = Zeta.Interleave
+module GV = Zeta.GenericVerifier
 
 (* a global log is a collection of thread-level verifier logs *)
 let vlog (vspec: verifier_spec) = seq (verifier_log vspec)
@@ -33,17 +35,56 @@ let clock #vspec (gl: verifiable_log vspec) (i: sseq_index gl) =
   let tl = thread_log gl tid in
   T.clock tl i'
 
-(* blum add set elements for a given epoch*)
-val add_set
+(* is a specified index a blum add? *)
+let is_blum_add #vspec (gl: verifiable_log vspec) (i: sseq_index gl): bool
+  = let tid, i' = i in
+    let tl = thread_log gl tid in
+    T.is_blum_add tl i'
+
+(* if an index is blum add, the blum add element for that index *)
+let blum_add_elem #vspec (gl: verifiable_log vspec) (i: sseq_index gl { is_blum_add gl i })
+  = let tid, i' = i in
+    let tl = thread_log gl tid in
+    T.blum_add_elem tl i'
+
+(* does a blum add belong to epoch ep*)
+let is_blum_add_in_epoch #vspec (ep: epoch) (gl: verifiable_log vspec) (i: sseq_index gl)
+  = let tid, i' = i in
+    let tl = thread_log gl tid in
+    T.is_blum_add_in_epoch ep tl i'
+
+(* blum add set elements for a given epoch *)
+let add_set
   (#vspec: verifier_spec)
   (ep: epoch)
   (gl: verifiable_log vspec): mset_ms_hashfn_dom vspec.app
+  = let f = is_blum_add_in_epoch ep gl in
+    let m = blum_add_elem gl in
+    sseq_indexed_filter_map_multiset (ms_hashfn_dom_cmp vspec.app) gl f m
+
+let is_blum_evict #vspec (gl: verifiable_log vspec) (i: sseq_index gl)
+  = let tid, i' = i in
+    let tl = thread_log gl tid in
+    T.is_blum_evict tl i'
+
+let blum_evict_elem #vspec (gl: verifiable_log vspec) (i: sseq_index gl { is_blum_evict gl i })
+  = let tid, i' = i in
+    let tl = thread_log gl tid in
+    T.blum_evict_elem tl i'
+
+let is_blum_evict_in_epoch #vspec (ep: epoch) (gl: verifiable_log vspec) (i: sseq_index gl)
+  = let tid, i' = i in
+    let tl = thread_log gl tid in
+    T.is_blum_evict_in_epoch ep tl i'
 
 (* blum evict set elements for a given epoch *)
-val evict_set
+let evict_set
   (#vspec: verifier_spec)
   (ep: epoch)
   (gl: verifiable_log vspec): mset_ms_hashfn_dom vspec.app
+  = let f = is_blum_evict_in_epoch ep gl in
+    let m = blum_evict_elem gl in
+    sseq_indexed_filter_map_multiset (ms_hashfn_dom_cmp vspec.app) gl f m
 
 (* verifiable log property that add- and evict sets are the same *)
 let aems_equal_for_epoch #vspec
