generic/Zeta.Generic.Thread.fst
@@ -36,66 +36,11 @@ let rec lemma_thread_id_state (#vspec:verifier_spec) (tl: verifiable_log vspec):
     if n = 0 then ()
     else lemma_thread_id_state (prefix tl (n-1))
 
-let add_epoch_filter #vspec (ep: epoch) (tl: verifiable_log vspec): ((seq_index tl) -> bool)
-  = let _,l = tl in
-    let f = fun (i: SA.seq_index l) ->
-            let e = S.index l i in
-            is_blum_add e &&
-            (let be = blum_add_elem e in
-            epoch_of be = ep) in
-    f
 
-let to_blum_add_elem #vspec (ep: epoch) (tl: verifiable_log vspec):
-  (i:seq_index tl{add_epoch_filter ep tl i} -> ms_hashfn_dom vspec.app)
-  = let _,l = tl in
-    let f = add_epoch_filter ep tl in
-    let m = fun (i: SA.seq_index l { f i }) ->
-            let e = S.index l i in
-            blum_add_elem e in
-    m
+let blum_add_elem (#vspec:_) (tl: verifiable_log vspec) (i: seq_index tl { is_blum_add tl i })
+  : ms_hashfn_dom vspec.app
+  = admit()
 
-let blum_add_seq (#vspec: verifier_spec) (ep: epoch) (tl: verifiable_log vspec):
-  S.seq (ms_hashfn_dom vspec.app)
-  = let _,l = tl in
-    let f = add_epoch_filter ep tl in
-    let m = to_blum_add_elem ep tl in
-    SA.indexed_filter_map l f m
-
-let add_seq_map
-  (#vspec: verifier_spec)
-  (tl: verifiable_log vspec)
-  (i: seq_index tl {is_blum_add (index tl i)}):
-  (let be = blum_add_elem (index tl i) in
-   let ep = epoch_of be in
-   let add_seq = blum_add_seq ep tl in
-   j: SA.seq_index add_seq{S.index add_seq j = be})
-  = let be = blum_add_elem (index tl i) in
-    let ep = epoch_of be in
-    let _,l = tl in
-    let f = add_epoch_filter ep tl in
-    let m = to_blum_add_elem ep tl in
-    SA.indexed_filter_map_map l f m i
-
-let add_seq_inv_map
-  (#vspec: verifier_spec)
-  (ep: epoch)
-  (tl: verifiable_log vspec)
-  (j: SA.seq_index (blum_add_seq ep tl)):
-  (i: seq_index tl {is_blum_add (index tl i) /\
-                    blum_add_elem (index tl i) = S.index (blum_add_seq ep tl) j /\
-                    epoch_of (blum_add_elem (index tl i)) = ep /\
-                    add_seq_map tl i = j})
- = let _,l = tl in
-   let f = add_epoch_filter ep tl in
-   let m = to_blum_add_elem ep tl in
-   SA.indexed_filter_map_invmap l f m j
-
-
-let lemma_add_seq_inv
-  (#vspec:_)
-  (tl: verifiable_log vspec)
-  (i: seq_index tl{is_blum_add (index tl i)}):
-  Lemma (ensures (let be = blum_add_elem (index tl i) in
-                  let ep = epoch_of be in
-                  add_seq_inv_map ep tl (add_seq_map tl i) = i))
-  = ()
+let blum_evict_elem (#vspec:_) (tl: verifiable_log vspec) (i: seq_index tl { is_blum_evict tl i }):
+  ms_hashfn_dom vspec.app
+  = admit()
