generic/Zeta.GenericVerifier.fst
@@ -1,0 +1,16 @@
+module Zeta.GenericVerifier
+
+let get_record_set (#vspec: verifier_spec_base) (ss: S.seq (vspec.slot_t)) (vtls: vspec.vtls_t {vspec.valid vtls}):
+  (let record_t = app_record vspec.app.adm in
+   ors: option (S.seq record_t) {Some? ors ==> (let rs = Some?.v ors in
+                                                S.length rs = S.length ss /\
+                                                distinct_keys #vspec.app.adm rs)})
+  = admit()
+
+
+let update_record_set (#vspec: verifier_spec_base)
+                      (ss: S.seq (vspec.slot_t))
+                      (vtls: vspec.vtls_t {vspec.valid vtls /\ Some? (get_record_set ss vtls)})
+                      (ws: S.seq (app_value_nullable vspec.app.adm) {let rs = get_record_set_succ ss vtls in
+                                                                     S.length ws = S.length rs}): vspec.vtls_t
+  = admit()
